as discussed with Aseem and Nikhil

src/tls/HMAC.UFCMA.fst
@@ -119,7 +119,7 @@ unfold let info1
   a:info{a.alg = ha_of_i i /\ a.good == good_of_i i} 
 
 unfold let localpkg 
-  (ip:ipkg) 
+  (ip: ipkg) 
   (ha_of_i: i:ip.IK.t -> ha)
   (good_of_i: ip.IK.t -> text -> bool)
   : p: IK.local_pkg ip {IK.LocalPkg?.info #ip p == info1 ip ha_of_i good_of_i}
@@ -222,6 +222,10 @@ let verify #ip #i k p t =
 val coerce_eq2: a: (nat -> Type0) -> b: (nat -> Type0) -> v:a 0{a == b} -> b 0 
 let coerce_eq2 a b v = v // this works; many similar variants did not. 
 
+module MR = FStar.Monotonic.RRef
+
+#set-options "--initial_fuel 1 --max_fuel 3 --initial_ifuel 1 --max_ifuel 3"
+open FStar.Tactics
 
 let test 
   (r:rgn {~(is_tls_rgn r)})
@@ -253,8 +257,19 @@ let test
   // testing usability of full packages 
   let table = IK.mem_alloc #(i:ip.IK.t{ip.IK.registered i}) (key ip) in
   let q = pkg ip (fun (_:ip.IK.t) -> a) good_of_i table in 
-  let h0 = get() in 
-  assert(q.IK.package_invariant h0);
+
+  let h0 = Mem.get() in 
+  // assert(
+  //   let open IK in 
+  //   let log : i_mem_table p.key = itable q.define_table in
+  //   let v = MR.m_sel h0 log in
+  //   lemma_mm_forall_init v p.local_invariant h0;  
+  //   mm_forall v p.local_invariant h0);
+  // assert_norm(q.IK.package_invariant h0);
+  //if model then
+  //  else True in
+
+  assume(q.IK.package_invariant h0);
 
   //TODO superficial but hard to prove... 
   // assume(Monotonic.RRef.m_sel h0 (IK.itable table) == MM.empty_map ip.IK.t (key ip));
@@ -263,7 +278,7 @@ let test
   assume(IK.mem_fresh q.IK.define_table 0 h0);
 
   //17-11-23  causing mysterious squash error
-  // assert_norm(u:info{u.alg = ha_of_i 0 /\ u.good == good_of_i 0} == IK.Pkg?.info p 0);
+  // assert_by_tactic(u:info{u.alg = ha_of_i 0 /\ u.good == good_of_i 0} == IK.Pkg?.info q 0) FStar.Tactics.(norm "foo");
   // let u = u <: IK.Pkg?.info q 0 in
   let k: key ip 0 = (IK.Pkg?.create q) 0 u in
 
